Switch to using pure_inline_relTheory

compiler/backend/passes/proofs/pure_inline_cexpProofScript.sml
@@ -12,21 +12,20 @@ open pure_expTheory pure_valueTheory pure_evalTheory pure_eval_lemmasTheory
      pure_letrec_seqTheory pure_demandTheory pure_dead_letProofTheory
      pure_letrecProofTheory;
 open pure_cexpTheory pure_varsTheory balanced_mapTheory pureLangTheory;
-open pure_inlineTheory pure_inline_cexpTheory pure_letrec_spec_cexpProofTheory
+open pure_inline_relTheory pure_inline_cexpTheory pure_letrec_spec_cexpProofTheory
      pure_barendregtTheory pure_freshenProofTheory var_setTheory;
 
 val _ = new_theory "pure_inline_cexpProof";
 
 Definition crhs_to_rhs_def:
-  crhs_to_rhs (cExp e) = (Exp $ exp_of e) ∧
-  crhs_to_rhs (cRec e) = (Rec $ exp_of e)
+  crhs_to_rhs (cExp e) = exp_of e
 End
 
 (* xs and m have the same elements *)
 Definition memory_inv_def:
   memory_inv xs m (ns:(mlstring,unit) map # num) ⇔
     { explode a | ∃e. lookup m a = SOME e } = set (MAP FST xs) ∧
-    EVERY (λ(v,r). v ∈ set_of ns ∧ ∃e:'a cexp. avoid_set_ok ns e ∧ r = Exp (exp_of e)) xs ∧
+    EVERY (λ(v,r). v ∈ set_of ns ∧ ∃e:'a cexp. avoid_set_ok ns e ∧ r = exp_of e) xs ∧
     ∀v e. (lookup m v = SOME e) ⇒
           ∃e1. e = cExp (e1:'a cexp) ∧ cheap e1 ∧
                MEM (explode v, (crhs_to_rhs e)) xs ∧
@@ -84,11 +83,11 @@ Proof
   \\ gvs []
 QED
 
-Theorem list_subst_rel_Apps:
+Theorem inline_rel_Apps:
   (∀ts us l t1 u1.
-    list_subst_rel l t1 u1 ∧
-    LIST_REL (list_subst_rel l) ts us ⇒
-    list_subst_rel l (Apps t1 ts) (Apps u1 us))
+    inline_rel l t1 u1 ∧
+    LIST_REL (inline_rel l) ts us ⇒
+    inline_rel l (Apps t1 ts) (Apps u1 us))
 Proof
   Induct
   >- fs [Apps_def]
@@ -96,7 +95,7 @@ Proof
   \\ rw []
   \\ last_x_assum irule
   \\ fs []
-  \\ irule list_subst_rel_App
+  \\ irule inline_rel_App
   \\ fs []
 QED
 
@@ -108,7 +107,7 @@ Theorem memory_inv_APPEND:
   letrecs_distinct (exp_of e1) ∧
   cexp_wf e1 ∧
   ¬MEM (explode v) (MAP FST xs) ⇒
-  memory_inv (xs ++ [(explode v,Exp (exp_of e1))]) (insert m v (cExp e1)) ns
+  memory_inv (xs ++ [(explode v,exp_of e1)]) (insert m v (cExp e1)) ns
 Proof
   gvs [memory_inv_def]
   \\ rw []
@@ -205,9 +204,9 @@ Proof
   \\ gvs []
 QED
 
-Theorem list_subst_rel_lets_for:
-  list_subst_rel xs a b ⇒
-  list_subst_rel xs
+Theorem inline_rel_lets_for:
+  inline_rel xs a b ⇒
+  inline_rel xs
     (lets_for c v vs a)
     (lets_for c v vs b)
 Proof
@@ -217,9 +216,9 @@ Proof
   \\ rw []
   \\ Cases_on `h`
   \\ fs [lets_for_def]
-  \\ irule list_subst_rel_App
-  \\ irule_at Any list_subst_rel_Lam
-  \\ fs [list_subst_rel_refl]
+  \\ irule inline_rel_App
+  \\ irule_at Any inline_rel_Lam
+  \\ fs [inline_rel_refl]
 QED
 
 Theorem lets_for_no_shadowing:
@@ -561,9 +560,9 @@ Proof
   \\ rpt conj_tac \\ rpt gen_tac \\ rpt disch_tac \\ rpt gen_tac \\ rpt disch_tac
   >~ [`Var _ _`] >- (
     gvs [inline_def]
-    \\ Cases_on `lookup m v` \\ gvs [list_subst_rel_refl]
-    \\ Cases_on `x` \\ gvs [list_subst_rel_refl]
-    \\ Cases_on `is_Lam c` \\ gvs [memory_inv_def,list_subst_rel_refl,exp_of_def]
+    \\ Cases_on `lookup m v` \\ gvs [inline_rel_refl]
+    \\ Cases_on `x` \\ gvs [inline_rel_refl]
+    \\ Cases_on `is_Lam c` \\ gvs [memory_inv_def,inline_rel_refl,exp_of_def]
     \\ Cases_on ‘cl = 0’ \\ gvs []
   )
   >~ [`App _ _ _`] >-
@@ -1495,11 +1494,11 @@ Proof
   strip_tac \\ drule $ cj 2 inline_wf_thm \\ fs [block_def]
 QED
 
-Theorem list_subst_rel_Lams:
-  ∀l t u w. list_subst_rel l t u ⇒ list_subst_rel l (Lams w t) (Lams w u)
+Theorem inline_rel_Lams:
+  ∀l t u w. inline_rel l t u ⇒ inline_rel l (Lams w t) (Lams w u)
 Proof
   Induct_on ‘w’ \\ fs [Lams_def] \\ rw []
-  \\ irule list_subst_rel_Lam
+  \\ irule inline_rel_Lam
   \\ res_tac \\ fs []
 QED
 
@@ -1759,7 +1758,6 @@ Proof
   \\ pop_assum kall_tac
   \\ Induct_on ‘xs’ \\ gvs [vars_of_def,freevars_of_def]
   \\ PairCases \\ fs []
-  \\ Cases_on ‘h1’ \\ fs []
   \\ gvs [vars_of_def,freevars_of_def]
   \\ rw [] \\ res_tac \\ fs []
   \\ imp_res_tac avoid_set_ok_set_of \\ fs []
@@ -1804,25 +1802,25 @@ Proof
   \\ gvs [pure_expTheory.letrecs_distinct_def] \\ rw []
 QED
 
-Theorem list_subst_rel_if_lemma:
-  list_subst_rel xs x y ⇒
-  list_subst_rel xs (if b then Seq Fail x else x) (if b then Seq Fail y else y)
+Theorem inline_rel_if_lemma:
+  inline_rel xs x y ⇒
+  inline_rel xs (if b then Seq Fail x else x) (if b then Seq Fail y else y)
 Proof
-  rw [] \\ irule list_subst_rel_Prim \\ gvs [list_subst_rel_refl]
+  rw [] \\ irule inline_rel_Prim \\ gvs [inline_rel_refl]
 QED
 
-Triviality list_subst_rel_rows_of:
+Triviality inline_rel_rows_of:
   ∀xs1 ys1.
-    list_subst_rel xs x y ∧
+    inline_rel xs x y ∧
     MAP FST xs1 = MAP FST ys1 ∧
     MAP (FST o SND) xs1 = MAP (FST o SND) ys1 ∧
-    LIST_REL (list_subst_rel xs) (MAP (SND o SND) xs1) (MAP (SND o SND) ys1) ⇒
-    list_subst_rel xs (rows_of v x xs1) (rows_of v y ys1)
+    LIST_REL (inline_rel xs) (MAP (SND o SND) xs1) (MAP (SND o SND) ys1) ⇒
+    inline_rel xs (rows_of v x xs1) (rows_of v y ys1)
 Proof
   Induct \\ Cases_on ‘ys1’ \\ gvs [rows_of_def]
   \\ PairCases_on ‘h’ \\ PairCases \\ gvs [rows_of_def] \\ rw []
-  \\ irule list_subst_rel_Prim \\ gvs [list_subst_rel_refl]
-  \\ irule list_subst_rel_lets_for \\ fs []
+  \\ irule inline_rel_Prim \\ gvs [inline_rel_refl]
+  \\ irule inline_rel_lets_for \\ fs []
 QED
 
 fun lemma () = inline_ind
@@ -1836,7 +1834,7 @@ fun lemma () = inline_ind
     no_shadowing (exp_of x) ∧
     DISJOINT (set (MAP FST xs)) (boundvars (exp_of x)) ∧
     (inline m ns cl h x) = (t, ns1) ⇒
-    list_subst_rel xs (exp_of x) (exp_of t)’
+    inline_rel xs (exp_of x) (exp_of t)’
   |> Q.SPEC ‘λm ns cl h es. ∀xs ts ns1.
     memory_inv xs m ns ∧
     map_ok m ∧
@@ -1848,10 +1846,10 @@ fun lemma () = inline_ind
     EVERY (λe. no_shadowing (exp_of e)) es ∧
     EVERY (λx. DISJOINT (set (MAP FST xs)) (boundvars (exp_of x))) es ∧
     (inline_list m ns cl h es) = (ts, ns1) ⇒
-    LIST_REL (λx t. list_subst_rel xs (exp_of x) (exp_of t)) es ts’
+    LIST_REL (λx t. inline_rel xs (exp_of x) (exp_of t)) es ts’
   |> CONV_RULE (DEPTH_CONV BETA_CONV);
 
-Theorem inline_cexp_list_subst_rel:
+Theorem inline_cexp_inline_rel:
   ^(lemma() |> concl |> rand)
 Proof
   match_mp_tac (lemma())
@@ -1859,21 +1857,22 @@ Proof
   \\ rpt (gen_tac ORELSE disch_tac)
   >~ [`Var _ _`] >- (
     Cases_on `inline m ns cl h (Var a v) = (Var a v, ns)`
-    >- gvs [list_subst_rel_refl,exp_of_def]
+    >- gvs [inline_rel_refl,exp_of_def]
     \\ gvs [inline_def]
-    \\ Cases_on `lookup m v` \\ gvs [list_subst_rel_refl]
-    \\ Cases_on `x` \\ gvs [list_subst_rel_refl]
-    \\ Cases_on `is_Lam c` \\ gvs [memory_inv_def,list_subst_rel_refl,exp_of_def]
+    \\ Cases_on `lookup m v` \\ gvs [inline_rel_refl]
+    \\ Cases_on `x` \\ gvs [inline_rel_refl]
+    \\ Cases_on `is_Lam c` \\ gvs [memory_inv_def,inline_rel_refl,exp_of_def]
     \\ Cases_on ‘cl = 0’ \\ gvs []
     \\ first_assum drule \\ strip_tac \\ fs []
     \\ gvs []
-    \\ irule_at Any list_subst_rel_Var
+    \\ irule_at Any inline_rel_Var
     \\ fs [crhs_to_rhs_def]
     \\ qpat_x_assum ‘MEM _ _’ $ irule_at Any
     \\ qexists_tac ‘exp_of c’ \\ fs [exp_eq_refl]
     \\ qsuff_tac ‘no_shadowing (exp_of c) ∧ boundvars (exp_of c) = {} ∧
                   NestedCase_free c ∧
-                  letrecs_distinct (exp_of c) ∧ cexp_wf c’ >- (res_tac \\ fs [])
+                  letrecs_distinct (exp_of c) ∧ cexp_wf c’
+    >- (res_tac \\ fs [pre_def])
     \\ fs []
     \\ Cases_on ‘c’ \\ gvs [cheap_def]
     \\ fs [exp_of_def,is_Lam_def,NULL_EQ]
@@ -1881,7 +1880,7 @@ Proof
   >~ [`App _ _ _`] >- (
     gvs [inline_def]
     \\ rpt (pairarg_tac \\ gvs [])
-    \\ gvs [list_subst_rel_refl,exp_of_def,SF ETA_ss]
+    \\ gvs [inline_rel_refl,exp_of_def,SF ETA_ss]
     \\ qspecl_then [`set (MAP FST xs)`,`exp_of e`,`MAP exp_of es`]
                    assume_tac DISJOINT_boundvars_Apps
     \\ drule no_shadowing_Apps_EVERY
@@ -1889,7 +1888,7 @@ Proof
     \\ Cases_on `get_Var_name e`
     >- (
       gvs [exp_of_def,SF ETA_ss]
-      \\ irule list_subst_rel_Apps
+      \\ irule inline_rel_Apps
       \\ fs [LIST_REL_MAP,o_DEF]
       \\ last_x_assum $ irule_at Any
       \\ last_x_assum $ irule_at Any
@@ -1906,7 +1905,7 @@ Proof
     \\ Cases_on `lookup m x`
     >- (
       gvs [exp_of_def,SF ETA_ss]
-      \\ irule list_subst_rel_Apps
+      \\ irule inline_rel_Apps
       \\ fs [LIST_REL_MAP,o_DEF]
       \\ last_x_assum $ irule_at Any
       \\ last_x_assum $ irule_at Any
@@ -1928,7 +1927,7 @@ Proof
     \\ reverse $ Cases_on `aa`
     >- (
       gvs [exp_of_def,SF ETA_ss]
-      \\ irule list_subst_rel_Apps
+      \\ irule inline_rel_Apps
       \\ fs [LIST_REL_MAP,o_DEF]
       \\ last_x_assum $ irule_at Any
       \\ last_x_assum $ irule_at Any
@@ -1950,12 +1949,12 @@ Proof
     \\ Cases_on `App_Lam_to_Lets q_fresh`
     >- (
       gvs [exp_of_def,SF ETA_ss]
-      \\ irule list_subst_rel_Apps
+      \\ irule inline_rel_Apps
       \\ fs [LIST_REL_MAP,o_DEF]
       \\ last_x_assum $ irule_at Any
       \\ gvs [memory_inv_def,DISJOINT_SYM]
       \\ fs [EVERY_MAP,DISJOINT_SYM]
-      \\ irule_at Any list_subst_rel_refl
+      \\ irule_at Any inline_rel_refl
       \\ fs [EVERY_MAP,DISJOINT_SYM,cexp_wf_def]
       \\ fs [EVERY_MEM,pure_expTheory.letrecs_distinct_def]
     )
@@ -1964,12 +1963,12 @@ Proof
     \\ Cases_on `cl = 0`
     >- (
       gvs [exp_of_def,SF ETA_ss]
-      \\ irule list_subst_rel_Apps
+      \\ irule inline_rel_Apps
       \\ fs [LIST_REL_MAP,o_DEF]
       \\ last_x_assum $ irule_at Any
       \\ gvs [memory_inv_def,DISJOINT_SYM]
       \\ fs [EVERY_MAP,DISJOINT_SYM]
-      \\ irule_at Any list_subst_rel_refl
+      \\ irule_at Any inline_rel_refl
       \\ fs [EVERY_MAP,DISJOINT_SYM,cexp_wf_def]
       \\ fs [EVERY_MEM,pure_expTheory.letrecs_distinct_def]
     )
@@ -1983,16 +1982,16 @@ Proof
     \\ rename [‘App_Lam_to_Lets (App a2 c2 l2)’]
     \\ Cases_on ‘c2’ \\ gvs [App_Lam_to_Lets_def]
     \\ rename [‘App a2 (Lam a3 l3 c3) es2’]
-    \\ irule list_subst_rel_trans
+    \\ irule inline_rel_trans
     \\ last_x_assum $ irule_at Any
-    \\ irule_at Any list_subst_rel_ExpEq
-    \\ irule_at (Pos hd) list_subst_rel_Apps
-    \\ irule_at (Pos hd) list_subst_rel_VarSimp
-    \\ ‘MEM (explode v,Exp (exp_of c)) xs’ by
+    \\ irule_at Any inline_rel_ExpEq
+    \\ irule_at (Pos hd) inline_rel_Apps
+    \\ irule_at (Pos hd) inline_rel_VarSimp
+    \\ ‘MEM (explode v,exp_of c) xs’ by
           (fs [memory_inv_def] \\ res_tac  \\ fs [crhs_to_rhs_def])
     \\ pop_assum $ irule_at Any
     \\ qexists_tac ‘MAP exp_of es1’
-    \\ gvs [LIST_REL_MAP]
+    \\ gvs [LIST_REL_MAP,pre_def]
     \\ rename [‘inline_list m ns cl h es = (es1,ns6)’]
     \\ drule pure_freshenProofTheory.freshen_cexp_correctness
     \\ impl_keep_tac
@@ -2121,7 +2120,7 @@ Proof
     \\ fs [heuristic_insert_def]
     \\ Cases_on `cheap e1 ∧ h e1`
     >- (
-      irule list_subst_rel_Let
+      irule inline_rel_Let
       \\ conj_tac
       >- (
         last_x_assum irule
@@ -2147,13 +2146,13 @@ Proof
     \\ full_simp_tac pure_ss []
     \\ pop_assum kall_tac
     \\ fs []
-    \\ irule list_subst_rel_App
+    \\ irule inline_rel_App
     \\ reverse $ conj_tac
     >- (
       last_x_assum irule
       \\ fs [DISJOINT_SYM,memory_inv_def,cexp_wf_def]
     )
-    \\ irule list_subst_rel_Lam
+    \\ irule inline_rel_Lam
     \\ last_x_assum irule
     \\ fs [DISJOINT_SYM]
     \\ imp_res_tac inline_set_of
@@ -2165,7 +2164,7 @@ Proof
   >~ [`Letrec _ _ _`] >- (
     gvs [inline_def]
     \\ rpt (pairarg_tac \\ gvs [])
-    \\ gvs [list_subst_rel_refl,exp_of_def]
+    \\ gvs [inline_rel_refl,exp_of_def]
     \\ fs [pure_expTheory.letrecs_distinct_def]
     \\ ‘avoid_set_ok ns e ∧ EVERY (avoid_set_ok ns o SND) vbs’ by
       (fs [avoid_set_ok_def,EVERY_MEM,exp_of_def,MEM_MAP,PULL_EXISTS,
@@ -2186,7 +2185,7 @@ Proof
     \\ gvs [MEM_MAP,PULL_EXISTS,FORALL_PROD,EVERY_MEM,cexp_wf_def]
     \\ Cases_on `heuristic_insert_Rec m h vbs = m`
     >- (
-      irule list_subst_rel_Letrec
+      irule inline_rel_Letrec
       \\ last_x_assum $ irule_at Any
       \\ gvs [] \\ fs [DISJOINT_SYM]
       \\ gvs [MAP_MAP_o,o_DEF,FORALL_PROD,LAMBDA_PROD,SND_intro,EVERY_MAP]
@@ -2210,7 +2209,7 @@ Proof
     \\ Cases_on ‘specialise w u’ \\ gvs []
     \\ fs [inline_def]
     \\ pairarg_tac \\ gvs []
-    \\ irule list_subst_rel_LetRecIntroExp
+    \\ irule inline_rel_LetRecIntroExp
     \\ conj_tac
     >- (
       last_x_assum $ irule_at Any
@@ -2256,7 +2255,7 @@ Proof
     gvs [inline_def,exp_of_def]
     \\ rpt (pairarg_tac \\ gvs [])
     \\ gvs [exp_of_def]
-    \\ irule_at Any list_subst_rel_Lams
+    \\ irule_at Any inline_rel_Lams
     \\ last_x_assum irule
     \\ imp_res_tac no_shadowing_Lams_e
     \\ fs [cexp_wf_def,letrecs_distinct_Lams]
@@ -2268,7 +2267,7 @@ Proof
     gvs [inline_def,exp_of_def]
     \\ rpt (pairarg_tac \\ gvs [])
     \\ gvs [inline_def,exp_of_def]
-    \\ irule list_subst_rel_Prim
+    \\ irule inline_rel_Prim
     \\ fs [LIST_REL_MAP,o_DEF,FORALL_PROD,LIST_REL_MAP2,PULL_EXISTS]
     \\ last_x_assum irule
     \\ fs [EVERY_MEM,cexp_wf_def,
@@ -2300,7 +2299,7 @@ Proof
       irule branch_vars_eq_lemma
       \\ gvs []
     )
-    \\ gvs [memory_inv_def,list_subst_rel_refl,exp_of_def,o_DEF]
+    \\ gvs [memory_inv_def,inline_rel_refl,exp_of_def,o_DEF]
     \\ gvs [MAP_MAP_o,o_DEF,FST,SND,MAP_ZIP,FST_intro]
     \\ sg `f = NONE ⇔ q'' = NONE`
     >- (
@@ -2420,8 +2419,8 @@ Proof
       \\ metis_tac []
     )
     \\ gvs [if_lemma]
-    \\ irule list_subst_rel_if_lemma
-    \\ irule list_subst_rel_App
+    \\ irule inline_rel_if_lemma
+    \\ irule inline_rel_App
     \\ reverse conj_tac
     >-
      (first_x_assum irule \\ fs []
@@ -2430,8 +2429,8 @@ Proof
       \\ first_x_assum (fn th => mp_tac th \\ match_mp_tac avoid_set_ok_subset_exp)
       \\ gvs [allvars_def,exp_of_def]
       \\ simp [SUBSET_DEF])
-    \\ irule list_subst_rel_Lam
-    \\ irule list_subst_rel_rows_of
+    \\ irule inline_rel_Lam
+    \\ irule inline_rel_rows_of
     \\ match_mp_tac (METIS_PROVE [] “(b1∧b2)∧(b3∧b4) ⇒ b1∧b2∧b3∧b4”)
     \\ conj_tac
     >-
@@ -2447,14 +2446,14 @@ Proof
     \\ reverse conj_tac
     >-
      (Cases_on ‘f’ \\ gvs []
-      >- (irule list_subst_rel_Prim \\ fs [])
+      >- (irule inline_rel_Prim \\ fs [])
       \\ PairCases_on ‘x’ \\ gvs []
       \\ rename [‘y ≠ NONE’] \\ Cases_on ‘y’ \\ gvs []
       \\ PairCases_on ‘x’ \\ gvs []
       \\ gvs [IfDisj_def]
-      \\ irule list_subst_rel_Prim \\ fs []
-      \\ irule_at Any list_subst_rel_Prim \\ fs []
-      \\ pairarg_tac \\ gvs [list_subst_rel_refl]
+      \\ irule inline_rel_Prim \\ fs []
+      \\ irule_at Any inline_rel_Prim \\ fs []
+      \\ pairarg_tac \\ gvs [inline_rel_refl]
       \\ last_x_assum irule \\ fs []
       \\ gvs [pure_expTheory.letrecs_distinct_def,
               letrecs_distinct_rows_of,cexp_wf_def]
@@ -2527,7 +2526,7 @@ Proof
   )
 QED
 
-Theorem inline_cexp_list_subst_rel_spec:
+Theorem inline_cexp_inline_rel_spec:
   ∀m ns cl h x xs t ns1.
     memory_inv xs m ns ∧
     map_ok m ∧ avoid_set_ok ns x ∧
@@ -2535,10 +2534,10 @@ Theorem inline_cexp_list_subst_rel_spec:
     no_shadowing (exp_of x) ∧
     DISJOINT (set (MAP FST xs)) (boundvars (exp_of x)) ∧
     (inline m ns cl h x) = (t, ns1) ⇒
-    list_subst_rel xs (exp_of x) (exp_of t)
+    inline_rel xs (exp_of x) (exp_of t)
 Proof
   rw []
-  \\ assume_tac inline_cexp_list_subst_rel
+  \\ assume_tac inline_cexp_inline_rel
   \\ gvs []
   \\ last_x_assum irule
   \\ gvs []
@@ -2559,8 +2558,8 @@ Proof
   \\ irule exp_eq_trans
   \\ irule_at (Pos last) (CONJUNCT1 $ SPEC_ALL dead_let_correct)
   \\ irule exp_eq_trans
-  \\ irule_at (Pos last) list_subst_rel_IMP_exp_eq
-  \\ irule_at Any inline_cexp_list_subst_rel_spec \\ fs []
+  \\ irule_at (Pos last) inline_rel_IMP_exp_eq
+  \\ irule_at Any inline_cexp_inline_rel_spec \\ fs []
   \\ pop_assum $ irule_at Any \\ fs []
   \\ fs [memory_inv_def]
   \\ drule pure_freshenProofTheory.freshen_cexp_correctness
